src/go_lang/StructTests.v
@@ -59,32 +59,4 @@ Section go_lang.
   Theorem baz_t : ⊢ three.baz : (three.T -> refT uint64T).
   Proof. typecheck. Qed.
 
-  Theorem load_ty_is1 : load_ty (uint64T * uint64T * uint64T)%ht "v" =
-                       (!"v", !("v" +ₗ #1), !("v" +ₗ #2))%E.
-  Proof.
-    cbv -[U64].
-    goal_is_exactly_equal.
-  Qed.
-
-  Theorem load_ty_is2 : load_ty (uint64T * (uint64T * uint64T) * uint64T)%ht "v" =
-                       (!"v", (!("v" +ₗ #1), !("v" +ₗ #1 +ₗ #1)), !("v" +ₗ #3))%E.
-  Proof.
-    cbv -[U64].
-    goal_is_exactly_equal.
-  Qed.
-
-  Theorem load_field_is1 : loadField three.S "bar" =
-                          (λ: "p", !("p" +ₗ #1))%V.
-  Proof.
-    cbv -[U64].
-    reflexivity.
-  Qed.
-
-  Theorem load_field_is2 : loadField three.S "baz" =
-                          (λ: "p", !("p" +ₗ #2))%V.
-  Proof.
-    cbv -[U64].
-    reflexivity.
-  Qed.
-
 End go_lang.
